---
layout: default
title : "Base.Homomorphisms.Products module (The Agda Universal Algebra Library)"
date : "2021-09-08"
author: "agda-algebras development team"
---

### <a id="products-of-homomorphisms">Products of Homomorphisms</a>

This is the [Base.Homomorphisms.Products] module of the [Agda Universal Algebra Library][].

<pre class="Agda">

<a id="345" class="Symbol">{-#</a> <a id="349" class="Keyword">OPTIONS</a> <a id="357" class="Pragma">--without-K</a> <a id="369" class="Pragma">--exact-split</a> <a id="383" class="Pragma">--safe</a> <a id="390" class="Symbol">#-}</a>

<a id="395" class="Keyword">open</a> <a id="400" class="Keyword">import</a> <a id="407" href="Base.Algebras.Basic.html" class="Module">Base.Algebras.Basic</a>

<a id="428" class="Keyword">module</a> <a id="435" href="Base.Homomorphisms.Products.html" class="Module">Base.Homomorphisms.Products</a> <a id="463" class="Symbol">{</a><a id="464" href="Base.Homomorphisms.Products.html#464" class="Bound">𝑆</a> <a id="466" class="Symbol">:</a> <a id="468" href="Base.Algebras.Basic.html#3888" class="Function">Signature</a> <a id="478" href="Base.Algebras.Basic.html#1160" class="Generalizable">𝓞</a> <a id="480" href="Base.Algebras.Basic.html#1162" class="Generalizable">𝓥</a><a id="481" class="Symbol">}</a> <a id="483" class="Keyword">where</a>

<a id="490" class="Comment">-- Imports from Agda and the Agda Standard Library --------------------------</a>
<a id="568" class="Keyword">open</a> <a id="573" class="Keyword">import</a> <a id="580" href="Agda.Primitive.html" class="Module">Agda.Primitive</a> <a id="595" class="Keyword">using</a> <a id="601" class="Symbol">(</a> <a id="603" href="Agda.Primitive.html#810" class="Primitive Operator">_⊔_</a> <a id="607" class="Symbol">;</a> <a id="609" href="Agda.Primitive.html#780" class="Primitive">lsuc</a> <a id="614" class="Symbol">)</a> <a id="616" class="Keyword">renaming</a> <a id="625" class="Symbol">(</a> <a id="627" href="Agda.Primitive.html#326" class="Primitive">Set</a> <a id="631" class="Symbol">to</a> <a id="634" class="Primitive">Type</a> <a id="639" class="Symbol">)</a>
<a id="641" class="Keyword">open</a> <a id="646" class="Keyword">import</a> <a id="653" href="Axiom.Extensionality.Propositional.html" class="Module">Axiom.Extensionality.Propositional</a>
                           <a id="715" class="Keyword">using</a> <a id="721" class="Symbol">()</a> <a id="724" class="Keyword">renaming</a> <a id="733" class="Symbol">(</a><a id="734" href="Axiom.Extensionality.Propositional.html#741" class="Function">Extensionality</a> <a id="749" class="Symbol">to</a> <a id="752" class="Function">funext</a><a id="758" class="Symbol">)</a>
<a id="760" class="Keyword">open</a> <a id="765" class="Keyword">import</a> <a id="772" href="Data.Product.html" class="Module">Data.Product</a>   <a id="787" class="Keyword">using</a> <a id="793" class="Symbol">(</a> <a id="795" href="Agda.Builtin.Sigma.html#236" class="InductiveConstructor Operator">_,_</a> <a id="799" class="Symbol">)</a>
<a id="801" class="Keyword">open</a> <a id="806" class="Keyword">import</a> <a id="813" href="Level.html" class="Module">Level</a>          <a id="828" class="Keyword">using</a> <a id="834" class="Symbol">(</a> <a id="836" href="Agda.Primitive.html#597" class="Postulate">Level</a> <a id="842" class="Symbol">)</a>
<a id="844" class="Keyword">open</a> <a id="849" class="Keyword">import</a> <a id="856" href="Relation.Binary.PropositionalEquality.html" class="Module">Relation.Binary.PropositionalEquality</a> <a id="894" class="Keyword">using</a> <a id="900" class="Symbol">(</a> <a id="902" href="Agda.Builtin.Equality.html#208" class="InductiveConstructor">refl</a> <a id="907" class="Symbol">)</a>

<a id="910" class="Comment">-- Imports from the Agda Universal Algebras Library ----------------------</a>
<a id="985" class="Keyword">open</a> <a id="990" class="Keyword">import</a> <a id="997" href="Base.Overture.Preliminaries.html" class="Module">Base.Overture.Preliminaries</a> <a id="1025" class="Keyword">using</a> <a id="1031" class="Symbol">(</a> <a id="1033" href="Base.Overture.Preliminaries.html#4402" class="Function Operator">∣_∣</a> <a id="1037" class="Symbol">;</a> <a id="1039" href="Base.Overture.Preliminaries.html#4440" class="Function Operator">∥_∥</a><a id="1042" class="Symbol">)</a>
<a id="1044" class="Keyword">open</a> <a id="1049" class="Keyword">import</a> <a id="1056" href="Base.Algebras.Products.html" class="Module">Base.Algebras.Products</a>    <a id="1082" class="Symbol">{</a><a id="1083" class="Argument">𝑆</a> <a id="1085" class="Symbol">=</a> <a id="1087" href="Base.Homomorphisms.Products.html#464" class="Bound">𝑆</a><a id="1088" class="Symbol">}</a> <a id="1090" class="Keyword">using</a> <a id="1096" class="Symbol">(</a> <a id="1098" href="Base.Algebras.Products.html#1899" class="Function">⨅</a> <a id="1100" class="Symbol">)</a>
<a id="1102" class="Keyword">open</a> <a id="1107" class="Keyword">import</a> <a id="1114" href="Base.Homomorphisms.Basic.html" class="Module">Base.Homomorphisms.Basic</a>  <a id="1140" class="Symbol">{</a><a id="1141" class="Argument">𝑆</a> <a id="1143" class="Symbol">=</a> <a id="1145" href="Base.Homomorphisms.Products.html#464" class="Bound">𝑆</a><a id="1146" class="Symbol">}</a> <a id="1148" class="Keyword">using</a> <a id="1154" class="Symbol">(</a> <a id="1156" href="Base.Homomorphisms.Basic.html#2682" class="Function">hom</a> <a id="1160" class="Symbol">;</a> <a id="1162" href="Base.Homomorphisms.Basic.html#4326" class="Function">epi</a> <a id="1166" class="Symbol">)</a>

<a id="1169" class="Keyword">private</a> <a id="1177" class="Keyword">variable</a> <a id="1186" href="Base.Homomorphisms.Products.html#1186" class="Generalizable">𝓘</a> <a id="1188" href="Base.Homomorphisms.Products.html#1188" class="Generalizable">β</a> <a id="1190" class="Symbol">:</a> <a id="1192" href="Agda.Primitive.html#597" class="Postulate">Level</a>

</pre>


Suppose we have an algebra `𝑨`, a type `I : Type 𝓘`, and a family `ℬ : I → Algebra β 𝑆` of algebras.  We sometimes refer to the inhabitants of `I` as *indices*, and call `ℬ` an *indexed family of algebras*.

If in addition we have a family `𝒽 : (i : I) → hom 𝑨 (ℬ i)` of homomorphisms, then we can construct a homomorphism from `𝑨` to the product `⨅ ℬ` in the natural way.

<pre class="Agda">

<a id="1600" class="Keyword">module</a> <a id="1607" href="Base.Homomorphisms.Products.html#1607" class="Module">_</a> <a id="1609" class="Symbol">{</a><a id="1610" href="Base.Homomorphisms.Products.html#1610" class="Bound">I</a> <a id="1612" class="Symbol">:</a> <a id="1614" href="Base.Homomorphisms.Products.html#634" class="Primitive">Type</a> <a id="1619" href="Base.Homomorphisms.Products.html#1186" class="Generalizable">𝓘</a><a id="1620" class="Symbol">}(</a><a id="1622" href="Base.Homomorphisms.Products.html#1622" class="Bound">ℬ</a> <a id="1624" class="Symbol">:</a> <a id="1626" href="Base.Homomorphisms.Products.html#1610" class="Bound">I</a> <a id="1628" class="Symbol">→</a> <a id="1630" href="Base.Algebras.Basic.html#6257" class="Function">Algebra</a> <a id="1638" href="Base.Homomorphisms.Products.html#1188" class="Generalizable">β</a> <a id="1640" href="Base.Homomorphisms.Products.html#464" class="Bound">𝑆</a><a id="1641" class="Symbol">)</a> <a id="1643" class="Keyword">where</a>

 <a id="1651" href="Base.Homomorphisms.Products.html#1651" class="Function">⨅-hom-co</a> <a id="1660" class="Symbol">:</a> <a id="1662" href="Base.Homomorphisms.Products.html#752" class="Function">funext</a> <a id="1669" href="Base.Homomorphisms.Products.html#1619" class="Bound">𝓘</a> <a id="1671" href="Base.Homomorphisms.Products.html#1638" class="Bound">β</a> <a id="1673" class="Symbol">→</a> <a id="1675" class="Symbol">{</a><a id="1676" href="Base.Homomorphisms.Products.html#1676" class="Bound">α</a> <a id="1678" class="Symbol">:</a> <a id="1680" href="Agda.Primitive.html#597" class="Postulate">Level</a><a id="1685" class="Symbol">}(</a><a id="1687" href="Base.Homomorphisms.Products.html#1687" class="Bound">𝑨</a> <a id="1689" class="Symbol">:</a> <a id="1691" href="Base.Algebras.Basic.html#6257" class="Function">Algebra</a> <a id="1699" href="Base.Homomorphisms.Products.html#1676" class="Bound">α</a> <a id="1701" href="Base.Homomorphisms.Products.html#464" class="Bound">𝑆</a><a id="1702" class="Symbol">)</a> <a id="1704" class="Symbol">→</a> <a id="1706" class="Symbol">(∀(</a><a id="1709" href="Base.Homomorphisms.Products.html#1709" class="Bound">i</a> <a id="1711" class="Symbol">:</a> <a id="1713" href="Base.Homomorphisms.Products.html#1610" class="Bound">I</a><a id="1714" class="Symbol">)</a> <a id="1716" class="Symbol">→</a> <a id="1718" href="Base.Homomorphisms.Basic.html#2682" class="Function">hom</a> <a id="1722" href="Base.Homomorphisms.Products.html#1687" class="Bound">𝑨</a> <a id="1724" class="Symbol">(</a><a id="1725" href="Base.Homomorphisms.Products.html#1622" class="Bound">ℬ</a> <a id="1727" href="Base.Homomorphisms.Products.html#1709" class="Bound">i</a><a id="1728" class="Symbol">))</a> <a id="1731" class="Symbol">→</a> <a id="1733" href="Base.Homomorphisms.Basic.html#2682" class="Function">hom</a> <a id="1737" href="Base.Homomorphisms.Products.html#1687" class="Bound">𝑨</a> <a id="1739" class="Symbol">(</a><a id="1740" href="Base.Algebras.Products.html#1899" class="Function">⨅</a> <a id="1742" href="Base.Homomorphisms.Products.html#1622" class="Bound">ℬ</a><a id="1743" class="Symbol">)</a>
 <a id="1746" href="Base.Homomorphisms.Products.html#1651" class="Function">⨅-hom-co</a> <a id="1755" href="Base.Homomorphisms.Products.html#1755" class="Bound">fe</a> <a id="1758" href="Base.Homomorphisms.Products.html#1758" class="Bound">𝑨</a> <a id="1760" href="Base.Homomorphisms.Products.html#1760" class="Bound">𝒽</a> <a id="1762" class="Symbol">=</a> <a id="1764" class="Symbol">(λ</a> <a id="1767" href="Base.Homomorphisms.Products.html#1767" class="Bound">a</a> <a id="1769" href="Base.Homomorphisms.Products.html#1769" class="Bound">i</a> <a id="1771" class="Symbol">→</a> <a id="1773" href="Base.Overture.Preliminaries.html#4402" class="Function Operator">∣</a> <a id="1775" href="Base.Homomorphisms.Products.html#1760" class="Bound">𝒽</a> <a id="1777" href="Base.Homomorphisms.Products.html#1769" class="Bound">i</a> <a id="1779" href="Base.Overture.Preliminaries.html#4402" class="Function Operator">∣</a> <a id="1781" href="Base.Homomorphisms.Products.html#1767" class="Bound">a</a><a id="1782" class="Symbol">)</a> <a id="1784" href="Agda.Builtin.Sigma.html#236" class="InductiveConstructor Operator">,</a> <a id="1786" class="Symbol">(λ</a> <a id="1789" href="Base.Homomorphisms.Products.html#1789" class="Bound">𝑓</a> <a id="1791" href="Base.Homomorphisms.Products.html#1791" class="Bound">𝒶</a> <a id="1793" class="Symbol">→</a> <a id="1795" href="Base.Homomorphisms.Products.html#1755" class="Bound">fe</a> <a id="1798" class="Symbol">λ</a> <a id="1800" href="Base.Homomorphisms.Products.html#1800" class="Bound">i</a> <a id="1802" class="Symbol">→</a> <a id="1804" href="Base.Overture.Preliminaries.html#4440" class="Function Operator">∥</a> <a id="1806" href="Base.Homomorphisms.Products.html#1760" class="Bound">𝒽</a> <a id="1808" href="Base.Homomorphisms.Products.html#1800" class="Bound">i</a> <a id="1810" href="Base.Overture.Preliminaries.html#4440" class="Function Operator">∥</a> <a id="1812" href="Base.Homomorphisms.Products.html#1789" class="Bound">𝑓</a> <a id="1814" href="Base.Homomorphisms.Products.html#1791" class="Bound">𝒶</a><a id="1815" class="Symbol">)</a>

</pre>

The family `𝒽` of homomorphisms inhabits the dependent type `Π i ꞉ I , hom 𝑨 (ℬ i)`.  The syntax we use to represent this type is available to us because of the way `-Π` is defined in the [Type Topology][] library.  We like this syntax because it is very close to the notation one finds in the standard type theory literature.  However,
we could equally well have used one of the following alternatives, which may be closer to "standard Agda" syntax:

`Π λ i → hom 𝑨 (ℬ i)` &nbsp; or &nbsp; `(i : I) → hom 𝑨 (ℬ i)` &nbsp; or &nbsp; `∀ i → hom 𝑨 (ℬ i)`.

The foregoing generalizes easily to the case in which the domain is also a product of a family of algebras. That is, if we are given `𝒜 : I → Algebra α 𝑆 and ℬ : I → Algebra β 𝑆` (two families of `𝑆`-algebras), and `𝒽 :  Π i ꞉ I , hom (𝒜 i)(ℬ i)` (a family of homomorphisms), then we can construct a homomorphism from `⨅ 𝒜` to `⨅ ℬ` in the following natural way.

<pre class="Agda">

 <a id="2763" href="Base.Homomorphisms.Products.html#2763" class="Function">⨅-hom</a> <a id="2769" class="Symbol">:</a> <a id="2771" href="Base.Homomorphisms.Products.html#752" class="Function">funext</a> <a id="2778" href="Base.Homomorphisms.Products.html#1619" class="Bound">𝓘</a> <a id="2780" href="Base.Homomorphisms.Products.html#1638" class="Bound">β</a> <a id="2782" class="Symbol">→</a> <a id="2784" class="Symbol">{</a><a id="2785" href="Base.Homomorphisms.Products.html#2785" class="Bound">α</a> <a id="2787" class="Symbol">:</a> <a id="2789" href="Agda.Primitive.html#597" class="Postulate">Level</a><a id="2794" class="Symbol">}(</a><a id="2796" href="Base.Homomorphisms.Products.html#2796" class="Bound">𝒜</a> <a id="2798" class="Symbol">:</a> <a id="2800" href="Base.Homomorphisms.Products.html#1610" class="Bound">I</a> <a id="2802" class="Symbol">→</a> <a id="2804" href="Base.Algebras.Basic.html#6257" class="Function">Algebra</a> <a id="2812" href="Base.Homomorphisms.Products.html#2785" class="Bound">α</a> <a id="2814" href="Base.Homomorphisms.Products.html#464" class="Bound">𝑆</a><a id="2815" class="Symbol">)</a> <a id="2817" class="Symbol">→</a> <a id="2819" class="Symbol">(∀</a> <a id="2822" class="Symbol">(</a><a id="2823" href="Base.Homomorphisms.Products.html#2823" class="Bound">i</a> <a id="2825" class="Symbol">:</a> <a id="2827" href="Base.Homomorphisms.Products.html#1610" class="Bound">I</a><a id="2828" class="Symbol">)</a> <a id="2830" class="Symbol">→</a> <a id="2832" href="Base.Homomorphisms.Basic.html#2682" class="Function">hom</a> <a id="2836" class="Symbol">(</a><a id="2837" href="Base.Homomorphisms.Products.html#2796" class="Bound">𝒜</a> <a id="2839" href="Base.Homomorphisms.Products.html#2823" class="Bound">i</a><a id="2840" class="Symbol">)</a> <a id="2842" class="Symbol">(</a><a id="2843" href="Base.Homomorphisms.Products.html#1622" class="Bound">ℬ</a> <a id="2845" href="Base.Homomorphisms.Products.html#2823" class="Bound">i</a><a id="2846" class="Symbol">))</a> <a id="2849" class="Symbol">→</a> <a id="2851" href="Base.Homomorphisms.Basic.html#2682" class="Function">hom</a> <a id="2855" class="Symbol">(</a><a id="2856" href="Base.Algebras.Products.html#1899" class="Function">⨅</a> <a id="2858" href="Base.Homomorphisms.Products.html#2796" class="Bound">𝒜</a><a id="2859" class="Symbol">)(</a><a id="2861" href="Base.Algebras.Products.html#1899" class="Function">⨅</a> <a id="2863" href="Base.Homomorphisms.Products.html#1622" class="Bound">ℬ</a><a id="2864" class="Symbol">)</a>
 <a id="2867" href="Base.Homomorphisms.Products.html#2763" class="Function">⨅-hom</a> <a id="2873" href="Base.Homomorphisms.Products.html#2873" class="Bound">fe</a> <a id="2876" href="Base.Homomorphisms.Products.html#2876" class="Bound">𝒜</a> <a id="2878" href="Base.Homomorphisms.Products.html#2878" class="Bound">𝒽</a> <a id="2880" class="Symbol">=</a> <a id="2882" class="Symbol">(λ</a> <a id="2885" href="Base.Homomorphisms.Products.html#2885" class="Bound">x</a> <a id="2887" href="Base.Homomorphisms.Products.html#2887" class="Bound">i</a> <a id="2889" class="Symbol">→</a> <a id="2891" href="Base.Overture.Preliminaries.html#4402" class="Function Operator">∣</a> <a id="2893" href="Base.Homomorphisms.Products.html#2878" class="Bound">𝒽</a> <a id="2895" href="Base.Homomorphisms.Products.html#2887" class="Bound">i</a> <a id="2897" href="Base.Overture.Preliminaries.html#4402" class="Function Operator">∣</a> <a id="2899" class="Symbol">(</a><a id="2900" href="Base.Homomorphisms.Products.html#2885" class="Bound">x</a> <a id="2902" href="Base.Homomorphisms.Products.html#2887" class="Bound">i</a><a id="2903" class="Symbol">))</a> <a id="2906" href="Agda.Builtin.Sigma.html#236" class="InductiveConstructor Operator">,</a> <a id="2908" class="Symbol">(λ</a> <a id="2911" href="Base.Homomorphisms.Products.html#2911" class="Bound">𝑓</a> <a id="2913" href="Base.Homomorphisms.Products.html#2913" class="Bound">𝒶</a> <a id="2915" class="Symbol">→</a> <a id="2917" href="Base.Homomorphisms.Products.html#2873" class="Bound">fe</a> <a id="2920" class="Symbol">λ</a> <a id="2922" href="Base.Homomorphisms.Products.html#2922" class="Bound">i</a> <a id="2924" class="Symbol">→</a> <a id="2926" href="Base.Overture.Preliminaries.html#4440" class="Function Operator">∥</a> <a id="2928" href="Base.Homomorphisms.Products.html#2878" class="Bound">𝒽</a> <a id="2930" href="Base.Homomorphisms.Products.html#2922" class="Bound">i</a> <a id="2932" href="Base.Overture.Preliminaries.html#4440" class="Function Operator">∥</a> <a id="2934" href="Base.Homomorphisms.Products.html#2911" class="Bound">𝑓</a> <a id="2936" class="Symbol">(λ</a> <a id="2939" href="Base.Homomorphisms.Products.html#2939" class="Bound">x</a> <a id="2941" class="Symbol">→</a> <a id="2943" href="Base.Homomorphisms.Products.html#2913" class="Bound">𝒶</a> <a id="2945" href="Base.Homomorphisms.Products.html#2939" class="Bound">x</a> <a id="2947" href="Base.Homomorphisms.Products.html#2922" class="Bound">i</a><a id="2948" class="Symbol">))</a>

</pre>


#### <a id="projections-out-of-products">Projection out of products</a>

Later we will need a proof of the fact that projecting out of a product algebra onto one of its factors is a homomorphism.

<pre class="Agda">

 <a id="3177" href="Base.Homomorphisms.Products.html#3177" class="Function">⨅-projection-hom</a> <a id="3194" class="Symbol">:</a> <a id="3196" class="Symbol">(</a><a id="3197" href="Base.Homomorphisms.Products.html#3197" class="Bound">i</a> <a id="3199" class="Symbol">:</a> <a id="3201" href="Base.Homomorphisms.Products.html#1610" class="Bound">I</a><a id="3202" class="Symbol">)</a> <a id="3204" class="Symbol">→</a> <a id="3206" href="Base.Homomorphisms.Basic.html#2682" class="Function">hom</a> <a id="3210" class="Symbol">(</a><a id="3211" href="Base.Algebras.Products.html#1899" class="Function">⨅</a> <a id="3213" href="Base.Homomorphisms.Products.html#1622" class="Bound">ℬ</a><a id="3214" class="Symbol">)</a> <a id="3216" class="Symbol">(</a><a id="3217" href="Base.Homomorphisms.Products.html#1622" class="Bound">ℬ</a> <a id="3219" href="Base.Homomorphisms.Products.html#3197" class="Bound">i</a><a id="3220" class="Symbol">)</a>
 <a id="3223" href="Base.Homomorphisms.Products.html#3177" class="Function">⨅-projection-hom</a> <a id="3240" class="Symbol">=</a> <a id="3242" class="Symbol">λ</a> <a id="3244" href="Base.Homomorphisms.Products.html#3244" class="Bound">x</a> <a id="3246" class="Symbol">→</a> <a id="3248" class="Symbol">(λ</a> <a id="3251" href="Base.Homomorphisms.Products.html#3251" class="Bound">z</a> <a id="3253" class="Symbol">→</a> <a id="3255" href="Base.Homomorphisms.Products.html#3251" class="Bound">z</a> <a id="3257" href="Base.Homomorphisms.Products.html#3244" class="Bound">x</a><a id="3258" class="Symbol">)</a> <a id="3260" href="Agda.Builtin.Sigma.html#236" class="InductiveConstructor Operator">,</a> <a id="3262" class="Symbol">λ</a> <a id="3264" href="Base.Homomorphisms.Products.html#3264" class="Bound">_</a> <a id="3266" href="Base.Homomorphisms.Products.html#3266" class="Bound">_</a> <a id="3268" class="Symbol">→</a> <a id="3270" href="Agda.Builtin.Equality.html#208" class="InductiveConstructor">refl</a>

</pre>

We could prove a more general result involving projections onto multiple factors, but so far the single-factor result has sufficed.

---------------------------------

<span style="float:left;">[← Base.Homomorphisms.Kernels](Base.Homomorphisms.Kernels.html)</span>
<span style="float:right;">[Base.Homomorphisms.Noether →](Base.Homomorphisms.Noether.html)</span>

{% include UALib.Links.md %}
