---
layout: default
title : "Homomorphisms.Products module (The Agda Universal Algebra Library)"
date : "2021-09-08"
author: "agda-algebras development team"
---

### <a id="products-of-homomorphisms">Products of Homomorphisms</a>

This is the [Homomorphisms.Products] module of the [Agda Universal Algebra Library][].

<pre class="Agda">

<a id="335" class="Symbol">{-#</a> <a id="339" class="Keyword">OPTIONS</a> <a id="347" class="Pragma">--without-K</a> <a id="359" class="Pragma">--exact-split</a> <a id="373" class="Pragma">--safe</a> <a id="380" class="Symbol">#-}</a>

<a id="385" class="Keyword">open</a> <a id="390" class="Keyword">import</a> <a id="397" href="Algebras.Basic.html" class="Module">Algebras.Basic</a>

<a id="413" class="Keyword">module</a> <a id="420" href="Homomorphisms.Products.html" class="Module">Homomorphisms.Products</a> <a id="443" class="Symbol">{</a><a id="444" href="Homomorphisms.Products.html#444" class="Bound">𝑆</a> <a id="446" class="Symbol">:</a> <a id="448" href="Algebras.Basic.html#3858" class="Function">Signature</a> <a id="458" href="Algebras.Basic.html#1130" class="Generalizable">𝓞</a> <a id="460" href="Algebras.Basic.html#1132" class="Generalizable">𝓥</a><a id="461" class="Symbol">}</a> <a id="463" class="Keyword">where</a>

<a id="470" class="Comment">-- Imports from Agda and the Agda Standard Library --------------------------</a>
<a id="548" class="Keyword">open</a> <a id="553" class="Keyword">import</a> <a id="560" href="Agda.Primitive.html" class="Module">Agda.Primitive</a> <a id="575" class="Keyword">using</a> <a id="581" class="Symbol">(</a> <a id="583" href="Agda.Primitive.html#810" class="Primitive Operator">_⊔_</a> <a id="587" class="Symbol">;</a> <a id="589" href="Agda.Primitive.html#780" class="Primitive">lsuc</a> <a id="594" class="Symbol">)</a> <a id="596" class="Keyword">renaming</a> <a id="605" class="Symbol">(</a> <a id="607" href="Agda.Primitive.html#326" class="Primitive">Set</a> <a id="611" class="Symbol">to</a> <a id="614" class="Primitive">Type</a> <a id="619" class="Symbol">)</a>
<a id="621" class="Keyword">open</a> <a id="626" class="Keyword">import</a> <a id="633" href="Axiom.Extensionality.Propositional.html" class="Module">Axiom.Extensionality.Propositional</a>
                           <a id="695" class="Keyword">using</a> <a id="701" class="Symbol">()</a> <a id="704" class="Keyword">renaming</a> <a id="713" class="Symbol">(</a><a id="714" href="Axiom.Extensionality.Propositional.html#741" class="Function">Extensionality</a> <a id="729" class="Symbol">to</a> <a id="732" class="Function">funext</a><a id="738" class="Symbol">)</a>
<a id="740" class="Keyword">open</a> <a id="745" class="Keyword">import</a> <a id="752" href="Data.Product.html" class="Module">Data.Product</a>   <a id="767" class="Keyword">using</a> <a id="773" class="Symbol">(</a> <a id="775" href="Agda.Builtin.Sigma.html#236" class="InductiveConstructor Operator">_,_</a> <a id="779" class="Symbol">)</a>
<a id="781" class="Keyword">open</a> <a id="786" class="Keyword">import</a> <a id="793" href="Level.html" class="Module">Level</a>          <a id="808" class="Keyword">using</a> <a id="814" class="Symbol">(</a> <a id="816" href="Agda.Primitive.html#597" class="Postulate">Level</a> <a id="822" class="Symbol">)</a>
<a id="824" class="Keyword">open</a> <a id="829" class="Keyword">import</a> <a id="836" href="Relation.Binary.PropositionalEquality.html" class="Module">Relation.Binary.PropositionalEquality</a> <a id="874" class="Keyword">using</a> <a id="880" class="Symbol">(</a> <a id="882" href="Agda.Builtin.Equality.html#208" class="InductiveConstructor">refl</a> <a id="887" class="Symbol">)</a>

<a id="890" class="Comment">-- Imports from the Agda Universal Algebras Library ----------------------</a>
<a id="965" class="Keyword">open</a> <a id="970" class="Keyword">import</a> <a id="977" href="Overture.Preliminaries.html" class="Module">Overture.Preliminaries</a> <a id="1000" class="Keyword">using</a> <a id="1006" class="Symbol">(</a> <a id="1008" href="Overture.Preliminaries.html#4382" class="Function Operator">∣_∣</a> <a id="1012" class="Symbol">;</a> <a id="1014" href="Overture.Preliminaries.html#4420" class="Function Operator">∥_∥</a><a id="1017" class="Symbol">)</a>
<a id="1019" class="Keyword">open</a> <a id="1024" class="Keyword">import</a> <a id="1031" href="Algebras.Products.html" class="Module">Algebras.Products</a>    <a id="1052" class="Symbol">{</a><a id="1053" class="Argument">𝑆</a> <a id="1055" class="Symbol">=</a> <a id="1057" href="Homomorphisms.Products.html#444" class="Bound">𝑆</a><a id="1058" class="Symbol">}</a> <a id="1060" class="Keyword">using</a> <a id="1066" class="Symbol">(</a> <a id="1068" href="Algebras.Products.html#1869" class="Function">⨅</a> <a id="1070" class="Symbol">)</a>
<a id="1072" class="Keyword">open</a> <a id="1077" class="Keyword">import</a> <a id="1084" href="Homomorphisms.Basic.html" class="Module">Homomorphisms.Basic</a>  <a id="1105" class="Symbol">{</a><a id="1106" class="Argument">𝑆</a> <a id="1108" class="Symbol">=</a> <a id="1110" href="Homomorphisms.Products.html#444" class="Bound">𝑆</a><a id="1111" class="Symbol">}</a> <a id="1113" class="Keyword">using</a> <a id="1119" class="Symbol">(</a> <a id="1121" href="Homomorphisms.Basic.html#2647" class="Function">hom</a> <a id="1125" class="Symbol">;</a> <a id="1127" href="Homomorphisms.Basic.html#4291" class="Function">epi</a> <a id="1131" class="Symbol">)</a>

<a id="1134" class="Keyword">private</a> <a id="1142" class="Keyword">variable</a> <a id="1151" href="Homomorphisms.Products.html#1151" class="Generalizable">𝓘</a> <a id="1153" href="Homomorphisms.Products.html#1153" class="Generalizable">β</a> <a id="1155" class="Symbol">:</a> <a id="1157" href="Agda.Primitive.html#597" class="Postulate">Level</a>

</pre>


Suppose we have an algebra `𝑨`, a type `I : Type 𝓘`, and a family `ℬ : I → Algebra β 𝑆` of algebras.  We sometimes refer to the inhabitants of `I` as *indices*, and call `ℬ` an *indexed family of algebras*.

If in addition we have a family `𝒽 : (i : I) → hom 𝑨 (ℬ i)` of homomorphisms, then we can construct a homomorphism from `𝑨` to the product `⨅ ℬ` in the natural way.

<pre class="Agda">

<a id="1565" class="Keyword">module</a> <a id="1572" href="Homomorphisms.Products.html#1572" class="Module">_</a> <a id="1574" class="Symbol">{</a><a id="1575" href="Homomorphisms.Products.html#1575" class="Bound">I</a> <a id="1577" class="Symbol">:</a> <a id="1579" href="Homomorphisms.Products.html#614" class="Primitive">Type</a> <a id="1584" href="Homomorphisms.Products.html#1151" class="Generalizable">𝓘</a><a id="1585" class="Symbol">}(</a><a id="1587" href="Homomorphisms.Products.html#1587" class="Bound">ℬ</a> <a id="1589" class="Symbol">:</a> <a id="1591" href="Homomorphisms.Products.html#1575" class="Bound">I</a> <a id="1593" class="Symbol">→</a> <a id="1595" href="Algebras.Basic.html#6222" class="Function">Algebra</a> <a id="1603" href="Homomorphisms.Products.html#1153" class="Generalizable">β</a> <a id="1605" href="Homomorphisms.Products.html#444" class="Bound">𝑆</a><a id="1606" class="Symbol">)</a> <a id="1608" class="Keyword">where</a>

 <a id="1616" href="Homomorphisms.Products.html#1616" class="Function">⨅-hom-co</a> <a id="1625" class="Symbol">:</a> <a id="1627" href="Homomorphisms.Products.html#732" class="Function">funext</a> <a id="1634" href="Homomorphisms.Products.html#1584" class="Bound">𝓘</a> <a id="1636" href="Homomorphisms.Products.html#1603" class="Bound">β</a> <a id="1638" class="Symbol">→</a> <a id="1640" class="Symbol">{</a><a id="1641" href="Homomorphisms.Products.html#1641" class="Bound">α</a> <a id="1643" class="Symbol">:</a> <a id="1645" href="Agda.Primitive.html#597" class="Postulate">Level</a><a id="1650" class="Symbol">}(</a><a id="1652" href="Homomorphisms.Products.html#1652" class="Bound">𝑨</a> <a id="1654" class="Symbol">:</a> <a id="1656" href="Algebras.Basic.html#6222" class="Function">Algebra</a> <a id="1664" href="Homomorphisms.Products.html#1641" class="Bound">α</a> <a id="1666" href="Homomorphisms.Products.html#444" class="Bound">𝑆</a><a id="1667" class="Symbol">)</a> <a id="1669" class="Symbol">→</a> <a id="1671" class="Symbol">(∀(</a><a id="1674" href="Homomorphisms.Products.html#1674" class="Bound">i</a> <a id="1676" class="Symbol">:</a> <a id="1678" href="Homomorphisms.Products.html#1575" class="Bound">I</a><a id="1679" class="Symbol">)</a> <a id="1681" class="Symbol">→</a> <a id="1683" href="Homomorphisms.Basic.html#2647" class="Function">hom</a> <a id="1687" href="Homomorphisms.Products.html#1652" class="Bound">𝑨</a> <a id="1689" class="Symbol">(</a><a id="1690" href="Homomorphisms.Products.html#1587" class="Bound">ℬ</a> <a id="1692" href="Homomorphisms.Products.html#1674" class="Bound">i</a><a id="1693" class="Symbol">))</a> <a id="1696" class="Symbol">→</a> <a id="1698" href="Homomorphisms.Basic.html#2647" class="Function">hom</a> <a id="1702" href="Homomorphisms.Products.html#1652" class="Bound">𝑨</a> <a id="1704" class="Symbol">(</a><a id="1705" href="Algebras.Products.html#1869" class="Function">⨅</a> <a id="1707" href="Homomorphisms.Products.html#1587" class="Bound">ℬ</a><a id="1708" class="Symbol">)</a>
 <a id="1711" href="Homomorphisms.Products.html#1616" class="Function">⨅-hom-co</a> <a id="1720" href="Homomorphisms.Products.html#1720" class="Bound">fe</a> <a id="1723" href="Homomorphisms.Products.html#1723" class="Bound">𝑨</a> <a id="1725" href="Homomorphisms.Products.html#1725" class="Bound">𝒽</a> <a id="1727" class="Symbol">=</a> <a id="1729" class="Symbol">(λ</a> <a id="1732" href="Homomorphisms.Products.html#1732" class="Bound">a</a> <a id="1734" href="Homomorphisms.Products.html#1734" class="Bound">i</a> <a id="1736" class="Symbol">→</a> <a id="1738" href="Overture.Preliminaries.html#4382" class="Function Operator">∣</a> <a id="1740" href="Homomorphisms.Products.html#1725" class="Bound">𝒽</a> <a id="1742" href="Homomorphisms.Products.html#1734" class="Bound">i</a> <a id="1744" href="Overture.Preliminaries.html#4382" class="Function Operator">∣</a> <a id="1746" href="Homomorphisms.Products.html#1732" class="Bound">a</a><a id="1747" class="Symbol">)</a> <a id="1749" href="Agda.Builtin.Sigma.html#236" class="InductiveConstructor Operator">,</a> <a id="1751" class="Symbol">(λ</a> <a id="1754" href="Homomorphisms.Products.html#1754" class="Bound">𝑓</a> <a id="1756" href="Homomorphisms.Products.html#1756" class="Bound">𝒶</a> <a id="1758" class="Symbol">→</a> <a id="1760" href="Homomorphisms.Products.html#1720" class="Bound">fe</a> <a id="1763" class="Symbol">λ</a> <a id="1765" href="Homomorphisms.Products.html#1765" class="Bound">i</a> <a id="1767" class="Symbol">→</a> <a id="1769" href="Overture.Preliminaries.html#4420" class="Function Operator">∥</a> <a id="1771" href="Homomorphisms.Products.html#1725" class="Bound">𝒽</a> <a id="1773" href="Homomorphisms.Products.html#1765" class="Bound">i</a> <a id="1775" href="Overture.Preliminaries.html#4420" class="Function Operator">∥</a> <a id="1777" href="Homomorphisms.Products.html#1754" class="Bound">𝑓</a> <a id="1779" href="Homomorphisms.Products.html#1756" class="Bound">𝒶</a><a id="1780" class="Symbol">)</a>

</pre>

The family `𝒽` of homomorphisms inhabits the dependent type `Π i ꞉ I , hom 𝑨 (ℬ i)`.  The syntax we use to represent this type is available to us because of the way `-Π` is defined in the [Type Topology][] library.  We like this syntax because it is very close to the notation one finds in the standard type theory literature.  However,
we could equally well have used one of the following alternatives, which may be closer to "standard Agda" syntax:

`Π λ i → hom 𝑨 (ℬ i)` &nbsp; or &nbsp; `(i : I) → hom 𝑨 (ℬ i)` &nbsp; or &nbsp; `∀ i → hom 𝑨 (ℬ i)`.

The foregoing generalizes easily to the case in which the domain is also a product of a family of algebras. That is, if we are given `𝒜 : I → Algebra α 𝑆 and ℬ : I → Algebra β 𝑆` (two families of `𝑆`-algebras), and `𝒽 :  Π i ꞉ I , hom (𝒜 i)(ℬ i)` (a family of homomorphisms), then we can construct a homomorphism from `⨅ 𝒜` to `⨅ ℬ` in the following natural way.

<pre class="Agda">

 <a id="2728" href="Homomorphisms.Products.html#2728" class="Function">⨅-hom</a> <a id="2734" class="Symbol">:</a> <a id="2736" href="Homomorphisms.Products.html#732" class="Function">funext</a> <a id="2743" href="Homomorphisms.Products.html#1584" class="Bound">𝓘</a> <a id="2745" href="Homomorphisms.Products.html#1603" class="Bound">β</a> <a id="2747" class="Symbol">→</a> <a id="2749" class="Symbol">{</a><a id="2750" href="Homomorphisms.Products.html#2750" class="Bound">α</a> <a id="2752" class="Symbol">:</a> <a id="2754" href="Agda.Primitive.html#597" class="Postulate">Level</a><a id="2759" class="Symbol">}(</a><a id="2761" href="Homomorphisms.Products.html#2761" class="Bound">𝒜</a> <a id="2763" class="Symbol">:</a> <a id="2765" href="Homomorphisms.Products.html#1575" class="Bound">I</a> <a id="2767" class="Symbol">→</a> <a id="2769" href="Algebras.Basic.html#6222" class="Function">Algebra</a> <a id="2777" href="Homomorphisms.Products.html#2750" class="Bound">α</a> <a id="2779" href="Homomorphisms.Products.html#444" class="Bound">𝑆</a><a id="2780" class="Symbol">)</a> <a id="2782" class="Symbol">→</a> <a id="2784" class="Symbol">(∀</a> <a id="2787" class="Symbol">(</a><a id="2788" href="Homomorphisms.Products.html#2788" class="Bound">i</a> <a id="2790" class="Symbol">:</a> <a id="2792" href="Homomorphisms.Products.html#1575" class="Bound">I</a><a id="2793" class="Symbol">)</a> <a id="2795" class="Symbol">→</a> <a id="2797" href="Homomorphisms.Basic.html#2647" class="Function">hom</a> <a id="2801" class="Symbol">(</a><a id="2802" href="Homomorphisms.Products.html#2761" class="Bound">𝒜</a> <a id="2804" href="Homomorphisms.Products.html#2788" class="Bound">i</a><a id="2805" class="Symbol">)</a> <a id="2807" class="Symbol">(</a><a id="2808" href="Homomorphisms.Products.html#1587" class="Bound">ℬ</a> <a id="2810" href="Homomorphisms.Products.html#2788" class="Bound">i</a><a id="2811" class="Symbol">))</a> <a id="2814" class="Symbol">→</a> <a id="2816" href="Homomorphisms.Basic.html#2647" class="Function">hom</a> <a id="2820" class="Symbol">(</a><a id="2821" href="Algebras.Products.html#1869" class="Function">⨅</a> <a id="2823" href="Homomorphisms.Products.html#2761" class="Bound">𝒜</a><a id="2824" class="Symbol">)(</a><a id="2826" href="Algebras.Products.html#1869" class="Function">⨅</a> <a id="2828" href="Homomorphisms.Products.html#1587" class="Bound">ℬ</a><a id="2829" class="Symbol">)</a>
 <a id="2832" href="Homomorphisms.Products.html#2728" class="Function">⨅-hom</a> <a id="2838" href="Homomorphisms.Products.html#2838" class="Bound">fe</a> <a id="2841" href="Homomorphisms.Products.html#2841" class="Bound">𝒜</a> <a id="2843" href="Homomorphisms.Products.html#2843" class="Bound">𝒽</a> <a id="2845" class="Symbol">=</a> <a id="2847" class="Symbol">(λ</a> <a id="2850" href="Homomorphisms.Products.html#2850" class="Bound">x</a> <a id="2852" href="Homomorphisms.Products.html#2852" class="Bound">i</a> <a id="2854" class="Symbol">→</a> <a id="2856" href="Overture.Preliminaries.html#4382" class="Function Operator">∣</a> <a id="2858" href="Homomorphisms.Products.html#2843" class="Bound">𝒽</a> <a id="2860" href="Homomorphisms.Products.html#2852" class="Bound">i</a> <a id="2862" href="Overture.Preliminaries.html#4382" class="Function Operator">∣</a> <a id="2864" class="Symbol">(</a><a id="2865" href="Homomorphisms.Products.html#2850" class="Bound">x</a> <a id="2867" href="Homomorphisms.Products.html#2852" class="Bound">i</a><a id="2868" class="Symbol">))</a> <a id="2871" href="Agda.Builtin.Sigma.html#236" class="InductiveConstructor Operator">,</a> <a id="2873" class="Symbol">(λ</a> <a id="2876" href="Homomorphisms.Products.html#2876" class="Bound">𝑓</a> <a id="2878" href="Homomorphisms.Products.html#2878" class="Bound">𝒶</a> <a id="2880" class="Symbol">→</a> <a id="2882" href="Homomorphisms.Products.html#2838" class="Bound">fe</a> <a id="2885" class="Symbol">λ</a> <a id="2887" href="Homomorphisms.Products.html#2887" class="Bound">i</a> <a id="2889" class="Symbol">→</a> <a id="2891" href="Overture.Preliminaries.html#4420" class="Function Operator">∥</a> <a id="2893" href="Homomorphisms.Products.html#2843" class="Bound">𝒽</a> <a id="2895" href="Homomorphisms.Products.html#2887" class="Bound">i</a> <a id="2897" href="Overture.Preliminaries.html#4420" class="Function Operator">∥</a> <a id="2899" href="Homomorphisms.Products.html#2876" class="Bound">𝑓</a> <a id="2901" class="Symbol">(λ</a> <a id="2904" href="Homomorphisms.Products.html#2904" class="Bound">x</a> <a id="2906" class="Symbol">→</a> <a id="2908" href="Homomorphisms.Products.html#2878" class="Bound">𝒶</a> <a id="2910" href="Homomorphisms.Products.html#2904" class="Bound">x</a> <a id="2912" href="Homomorphisms.Products.html#2887" class="Bound">i</a><a id="2913" class="Symbol">))</a>

</pre>


#### <a id="projections-out-of-products">Projection out of products</a>

Later we will need a proof of the fact that projecting out of a product algebra onto one of its factors is a homomorphism.

<pre class="Agda">

 <a id="3142" href="Homomorphisms.Products.html#3142" class="Function">⨅-projection-hom</a> <a id="3159" class="Symbol">:</a> <a id="3161" class="Symbol">(</a><a id="3162" href="Homomorphisms.Products.html#3162" class="Bound">i</a> <a id="3164" class="Symbol">:</a> <a id="3166" href="Homomorphisms.Products.html#1575" class="Bound">I</a><a id="3167" class="Symbol">)</a> <a id="3169" class="Symbol">→</a> <a id="3171" href="Homomorphisms.Basic.html#2647" class="Function">hom</a> <a id="3175" class="Symbol">(</a><a id="3176" href="Algebras.Products.html#1869" class="Function">⨅</a> <a id="3178" href="Homomorphisms.Products.html#1587" class="Bound">ℬ</a><a id="3179" class="Symbol">)</a> <a id="3181" class="Symbol">(</a><a id="3182" href="Homomorphisms.Products.html#1587" class="Bound">ℬ</a> <a id="3184" href="Homomorphisms.Products.html#3162" class="Bound">i</a><a id="3185" class="Symbol">)</a>
 <a id="3188" href="Homomorphisms.Products.html#3142" class="Function">⨅-projection-hom</a> <a id="3205" class="Symbol">=</a> <a id="3207" class="Symbol">λ</a> <a id="3209" href="Homomorphisms.Products.html#3209" class="Bound">x</a> <a id="3211" class="Symbol">→</a> <a id="3213" class="Symbol">(λ</a> <a id="3216" href="Homomorphisms.Products.html#3216" class="Bound">z</a> <a id="3218" class="Symbol">→</a> <a id="3220" href="Homomorphisms.Products.html#3216" class="Bound">z</a> <a id="3222" href="Homomorphisms.Products.html#3209" class="Bound">x</a><a id="3223" class="Symbol">)</a> <a id="3225" href="Agda.Builtin.Sigma.html#236" class="InductiveConstructor Operator">,</a> <a id="3227" class="Symbol">λ</a> <a id="3229" href="Homomorphisms.Products.html#3229" class="Bound">_</a> <a id="3231" href="Homomorphisms.Products.html#3231" class="Bound">_</a> <a id="3233" class="Symbol">→</a> <a id="3235" href="Agda.Builtin.Equality.html#208" class="InductiveConstructor">refl</a>

</pre>

We could prove a more general result involving projections onto multiple factors, but so far the single-factor result has sufficed.

---------------------------------

<span style="float:left;">[← Homomorphisms.Kernels](Homomorphisms.Kernels.html)</span>
<span style="float:right;">[Homomorphisms.Noether →](Homomorphisms.Noether.html)</span>

{% include UALib.Links.md %}
